Semantic safety for iolang

theories/input_lang/logpred.v
@@ -225,3 +225,65 @@ Section io_lang.
   Proof. apply fundamental. Qed.
 
 End io_lang.
+
+Local Definition rs : gReifiers _ := gReifiers_cons reify_io gReifiers_nil.
+
+Variable Hdisj : ∀ (Σ : gFunctors) (P Q : iProp Σ), disjunction_property P Q.
+
+Lemma logpred_adequacy τ (α : unitO -n> IT (gReifiers_ops rs)) (β : IT (gReifiers_ops rs)) st st' k :
+  (∀ {Σ:gFunctors}`{H1 : !invGS Σ} `{H2: !stateG rs Σ},
+      (True ⊢ valid1 rs notStuck (λ _:unitO, True)%I empC α τ)%I) →
+  ssteps (gReifiers_sReifier rs) (α ()) st β st' k →
+  (∃ β1 st1, sstep (gReifiers_sReifier rs) β st' β1 st1)
+   ∨ (∃ βv, IT_of_V βv ≡ β).
+Proof.
+  intros Hlog Hst.
+  destruct (IT_to_V β) as [βv|] eqn:Hb.
+  { right. exists βv. apply IT_of_to_V'. rewrite Hb; eauto. }
+  left.
+  cut ((∃ β1 st1, sstep (gReifiers_sReifier rs) β st' β1 st1)
+      ∨ (∃ e, β ≡ Err e ∧ notStuck e)).
+  { intros [?|He]; first done.
+    destruct He as [? [? []]]. }
+  eapply wp_safety; eauto.
+  { apply Hdisj. }
+  { by rewrite Hb. }
+  intros Σ H1 H2.
+  exists (interp_ty _ notStuck (λ _:unitO, True) τ)%I. split.
+  { apply _. }
+  iIntros "Hst".
+  iPoseProof (Hlog with "[//]") as "Hlog".
+  destruct st as [σ []].
+  iAssert (has_substate σ) with "[Hst]" as "Hs".
+  { unfold has_substate, has_full_state.
+    assert (of_state rs (IT (gReifiers_ops rs)) (σ,()) ≡
+            of_idx rs (IT (gReifiers_ops rs)) sR_idx (sR_state σ)) as ->; last done.
+    intro j. unfold sR_idx. simpl.
+    unfold of_state, of_idx.
+    destruct decide as [Heq|]; last first.
+    { inv_fin j; first done.
+      intros i. inversion i. }
+    inv_fin j; last done.
+    intros Heq.
+    rewrite (eq_pi _ _ Heq eq_refl)//.
+  }
+  iSpecialize ("Hlog" $! σ with "Hs []").
+  { iApply ssubst_valid_nil. }
+  iSpecialize ("Hlog" $! tt with "[//]").
+  iApply (wp_wand with"Hlog").
+  iIntros ( βv). simpl. iDestruct 1 as (_) "[H _]".
+  iDestruct "H" as (σ1') "[$ Hsts]".
+  done.
+Qed.
+
+Lemma io_lang_safety e τ σ st' β k :
+  typed empC e τ →
+  ssteps (gReifiers_sReifier rs) (interp_expr _ e ()) (σ,()) β st' k →
+  (∃ β1 st1, sstep (gReifiers_sReifier rs) β st' β1 st1)
+   ∨ (∃ βv, IT_of_V βv ≡ β).
+Proof.
+  intros Htyped Hsteps.
+  eapply logpred_adequacy; eauto.
+  intros Σ ? ?. iIntros "_".
+  by iApply fundamental.
+Qed.
